project3/strings3_vas_preds.dfy
@@ -1,0 +1,151 @@
+/*
+	isPrefix
+*/
+predicate isPrefixPred(pre:string, str:string) {
+	|pre| > 0 && (|pre| <= |str|) && pre == str[..|pre|]
+}
+
+predicate isNotPrefixPred(pre:string, str:string) {
+	|pre| <= 0 || (|pre| > |str|) || pre != str[..|pre|]
+}
+
+lemma PrefixNegationLemma(pre:string, str:string)
+	ensures  isPrefixPred(pre,str) <==> !isNotPrefixPred(pre,str)
+	ensures !isPrefixPred(pre,str) <==>  isNotPrefixPred(pre,str)
+{}
+
+method isPrefix(pre: string, str: string) returns (res:bool)
+	ensures !res <==> isNotPrefixPred(pre,str)
+	ensures  res <==> isPrefixPred(pre,str)
+{
+	if (|pre| > |str| || |pre| <= 0) {
+		return false;
+	}
+
+	return str[..|pre|] == pre;
+}
+
+
+
+
+
+
+/*
+	isSubstring
+*/
+predicate isSubstringPred(sub:string, str:string) {
+	(0 < |sub| <= |str|) && (exists i :: 0 <= i <= |str| - |sub| &&  isPrefixPred(sub, str[i..]))
+}
+
+predicate isNotSubstringPred(sub:string, str:string) {
+	!(0 < |sub| <= |str|) || (forall i :: 0 <= i <= |str| - |sub| ==> isNotPrefixPred(sub,str[i..]))
+}
+
+lemma SubstringNegationLemma(sub:string, str:string)
+	ensures  isSubstringPred(sub,str) <==> !isNotSubstringPred(sub,str)
+	ensures !isSubstringPred(sub,str) <==>  isNotSubstringPred(sub,str)
+{}
+
+// This should probably hold..
+/*
+lemma PrefixImpliesSubstringLemma(pre:string, str:string)
+	ensures isPrefixPred(pre, str) ==> isSubstringPred(pre, str)
+	ensures isNotSubstringPred(pre, str) ==> isNotPrefixPred(pre, str)
+{}*/
+
+// This holds for res ==> isSubstr and isNotRes  ==> !res
+// Doesn't hold for other way arounds though
+method isSubstring(sub: string, str: string) returns (res:bool)
+	ensures  res ==> isSubstringPred(sub, str)
+	//ensures isSubstringPred(sub, str) ==> res
+
+	//ensures !res ==> isNotSubstringPred(sub, str)
+	ensures isNotSubstringPred(sub, str) ==> !res
+
+{
+
+	if !(0 < |sub| <= |str|) {
+		return false;
+	}
+
+	var i := 0;
+	res := false;
+	while (i <= |str| - |sub|)
+	// If we don't quick exit the loop, its not a substring
+	invariant (i > |str| - |sub|) ==> (res == false)
+	//invariant (i > |str| - |sub|) ==> isNotSubstringPred(sub, str))
+	{
+		var tail := str[i..];
+		var isAPrefix := isPrefix(sub, tail);
+		if (isAPrefix) {
+			// These might help dafny choose a value for the existential..
+			assert isPrefixPred(sub, str[i..]);
+			assert isSubstringPred(sub, str);
+			return true;
+		}
+
+		i := i + 1;
+	}
+
+	//assert isNotSubstringPred(sub, str);
+	return false;
+}
+
+
+
+
+
+
+
+/*
+	K Substring
+*/
+predicate haveCommonKSubstringPred(k:nat, str1:string, str2:string) {
+	exists i1, j1 :: 0 <= i1 <= |str1|- k && j1 == i1 + k && isSubstringPred(str1[i1..j1],str2)
+}
+
+predicate haveNotCommonKSubstringPred(k:nat, str1:string, str2:string) {
+	forall i1, j1 :: 0 <= i1 <= |str1|- k && j1 == i1 + k ==>  isNotSubstringPred(str1[i1..j1],str2)
+}
+
+lemma commonKSubstringLemma(k:nat, str1:string, str2:string)
+	ensures  haveCommonKSubstringPred(k,str1,str2) <==> !haveNotCommonKSubstringPred(k,str1,str2)
+	ensures !haveCommonKSubstringPred(k,str1,str2) <==>  haveNotCommonKSubstringPred(k,str1,str2)
+{}
+
+method haveCommonKSubstring(k: nat, str1: string, str2: string) returns (found: bool)
+	ensures found  ==>  haveCommonKSubstringPred(k,str1,str2)
+	ensures haveCommonKSubstringPred(k,str1,str2) ==> found
+	//ensures !found <==> haveNotCommonKSubstringPred(k,str1,str2) // This postcondition follows from the above lemma.
+{
+// If either strings are smaller than k, they have no common substring of size k
+	if (|str1| < k || |str2| < k) {
+		assert haveNotCommonKSubstringPred(k, str1, str2);
+		return false;
+	}
+
+	// Create each substring of size k from str1
+	var startIndex := 0;
+	while (startIndex <= |str1| - k) 
+	
+	{
+		var endIndex := startIndex + k;
+
+		// Ensure largest index is the number of elements in sequence
+		// It can reach the number of elements in the sequence as slice is closed at end of interval 
+		assert endIndex <= |str1|;
+
+		// Get a substring of length k from str1							
+		var substr := str1[startIndex..endIndex];
+		assert |substr| == k;
+
+		var isSubstr := isSubstring(substr, str2);
+		if (isSubstr) {
+			return true;
+		}
+
+		startIndex := startIndex + 1;
+	}
+
+	return false;
+}
